done/Iron/Data/List/Concat.v
@@ -1,0 +1,11 @@
+
+Require Import Iron.Data.List.Base.
+
+
+Fixpoint catOptions {A} (xs : list (option A)) : list A
+ := match xs with
+    | nil             => nil
+    | Some x :: rest  => x :: catOptions rest
+    | None   :: rest  => catOptions rest
+    end.
+
