done/Iron/Data/List/Elem.v
@@ -1,0 +1,43 @@
+
+Require Import Iron.Data.List.Base.
+
+
+(* Check if any element in a list matches the given predicate. *)
+Fixpoint elem {A} (p : A -> bool) (xx : list A)
+ := match xx with
+    | nil      => false
+    | x :: xs  => if p x then true else elem p xs
+    end.
+
+
+Lemma elem_get_not
+ :  forall {A} (p : A -> bool) (xx : list A) 
+ ,  not (exists ix x, get ix xx = Some x /\ p x = true)
+ -> elem p xx = false.
+Proof. 
+ intros.
+ induction xx.
+ - simpl. auto.
+ - remember (p a) as X.
+   destruct X.
+   + simpl. 
+     rewrite <- HeqX.
+     assert (exists ix x, get ix (xx :> a) = Some x /\ p x = true).
+      exists 0. exists a. intuition.
+     tauto.
+     
+   + simpl. 
+     rewrite <- HeqX. 
+     eapply IHxx.
+     unfold not. 
+     intros.
+     destruct H0 as [ix].
+     destruct H0 as [x].
+     inversion H0.
+     assert (get (S ix) (xx :> a) = Some x).
+      simpl. auto.
+     assert (exists ix x, get ix (xx :> a) = Some x /\ p x = true).
+      exists (S ix). exists x. auto.
+     tauto.
+Qed.  
+
